fairness/lawyer/obligations/gset_prod.v
@@ -1,0 +1,16 @@
+From stdpp Require Export sets. 
+From iris.proofmode Require Import tactics.
+
+
+Section GsetProd.
+  Context `{Countable K, Countable T}. 
+
+  (* TODO: move / find implementation *)
+  Definition gset_prod (k: gset K) (t: gset T): gset (K * T).
+  Admitted.
+
+  Lemma gset_prod_spec (k: gset K) (t: gset T):
+    forall p, p ∈ gset_prod k t <-> p.1 ∈ k /\ p.2 ∈ t.
+  Proof using. Admitted.
+
+End GsetProd.
